FiatFormal/Language/Base.v
@@ -7,3 +7,5 @@ Require Export FiatFormal.Tactics.Have.
 Require Export FiatFormal.Tactics.Rip2.
 Require Export Coq.Program.Basics.
 Require Export Coq.Arith.Compare_dec.
+
+Require Export FiatFormal.PMKTactics.
