FiatFormal/Language/PreservationP.v
@@ -1,0 +1,95 @@
+
+Require Import FiatFormal.Language.Step.
+Require Import FiatFormal.Language.SubstExpExp.
+Require Import FiatFormal.Language.SubstTypeExp.
+Require Import FiatFormal.Language.SubstTypeType.
+Require Import FiatFormal.Language.TyJudge.
+
+
+(* When a program takes a step the results has the same type. *)
+Theorem preservationP
+ :  forall ke te p p' t
+ ,  TYPEPROG ke te p t
+ -> STEPP p p'
+ -> TYPEPROG ke te p' t.
+Proof.
+  intros ke te x x' t HT HS.
+  gen ke te x' t.
+  induction x; intros.
+  Case "PLet".
+  invert HS; intros.
+
+
+ intros ke te x x' t HT HS.
+ gen ke te x' t.
+ induction x; intros.
+
+ Case "XVar".
+  inverts HS.
+
+ Case "XLAM".
+  inverts HS.
+
+ Case "XAPP".
+  inverts HT.
+  inverts keep HS.
+
+  SCase "ESAPPLAM".
+   inverts H3.
+   eapply subst_type_value in H4; eauto.
+   rewrite substTE_liftTE in H4. auto.
+
+  SCase "ESAPP1".
+   apply TYAPP; eauto.
+
+ Case "XLam".
+  inverts HS.
+
+ Case "XApp".
+  inverts HT.
+  inverts keep HS.
+
+  SCase "ESAppLam".
+   inverts H3.
+   lets D: subst_value_value H9 H5. auto.
+
+  SCase "EsApp1".
+   eapply TYApp; eauto.
+
+  SCase "EsApp2".
+   eapply TYApp; eauto.
+Qed.
+
+
+(* When we multi-step evaluate some expression,
+   then the result has the same type as the original.
+ *)
+Lemma preservation_steps
+ :  forall x1 t1 x2
+ ,  TYPE nil nil x1 t1
+ -> STEPS x1 x2
+ -> TYPE nil nil x2 t1.
+Proof.
+ intros.
+ induction H0; eauto.
+  eapply preservation; eauto.
+Qed.
+
+
+(* When we multi-step evaluate some expression,
+   then the result has the same type as the original.
+   Using the left-linearised form for the evaluation.
+ *)
+Lemma preservation_stepsl
+ :  forall x1 t1 x2
+ ,  TYPE nil nil x1 t1
+ -> STEPSL x1 x2
+ -> TYPE nil nil x2 t1.
+Proof.
+ intros.
+ induction H0.
+  auto.
+  apply IHSTEPSL.
+  eapply preservation.
+   eauto. auto.
+Qed.
