FiatFormal/Language/ProgressP.v
@@ -1,0 +1,89 @@
+
+Require Import FiatFormal.Language.Step.
+Require Import FiatFormal.Language.SubstExpExp.
+Require Import FiatFormal.Language.SubstTypeExp.
+Require Import FiatFormal.Language.SubstTypeType.
+Require Import FiatFormal.Language.TyJudge.
+Require Import FiatFormal.Language.Progress.
+
+(* A well typed program is either a value, can take a step, or has a choice. *)
+Theorem progressP
+  : forall p,
+    (exists t, TYPEPROG nil nil p t)
+    -> valueP p \/ (exists p', STEPP p p'). (* \/ hasChoiceP p. *)
+Proof.
+  intros.
+  induction p.
+  Case "PLet".
+  right.
+  destruct H as [tp].
+  inverts H.
+  invert_adt_type.
+  eexists.
+  eapply SP_Prog.
+  Case "PExp".
+  inverts H.
+  invert_prog_type.
+  rename x into t.
+  pose proof (progress e).
+  destruct H. eexists. eassumption. (* TODO: ask ben why ex_spec *)
+                                (* doesn't match here *)
+  left; repeat constructor.
+  inversion H; auto.
+  unfold closedP. simpl.
+  inversion H. unfold closedX in *. assumption. (* TODO: ask ben how *)
+  (* to write Ltac to automate this *)
+  right. dest H. exists (PEXP x'). auto.
+Qed.
+
+(*  intros. *)
+(*  induction p; destruct H as [tx]. *)
+
+(*  Case "XVar". *)
+(*   inverts H. false. *)
+
+(*  Case "XLAM". *)
+(*   left. apply type_wfX in H. auto. *)
+
+(*  Case "XAPP". *)
+(*   inverts H. *)
+(*   destruct IHx. eauto. *)
+(*   SCase "x value". *)
+(*    right. inverts H. inverts H4. *)
+(*     inverts H1. false. *)
+(*     inverts H0. *)
+(*     exists (substTX 0 t x1). eapply ESLAMAPP. *)
+(*     inverts H0. *)
+(*   SCase "x steps". *)
+(*    right. *)
+(*     destruct H as [x']. *)
+(*     exists (XAPP x' t). *)
+(*     apply ESAPP1. auto. *)
+
+(*  Case "XLam". *)
+(*   left. apply type_wfX in H. auto. *)
+
+(*  Case "XApp". *)
+(*   right. *)
+(*   inverts H. *)
+(*   destruct IHx1; eauto. *)
+(*   SCase "x1 value". *)
+(*    destruct IHx2; eauto. *)
+(*    inverts H. *)
+
+(*    SSCase "x2 value". *)
+(*     inverts H1. *)
+(*      inverts H2. false. *)
+(*      inverts H4. *)
+(*      exists (substXX 0 x2 x0). apply ESLamApp. auto. *)
+
+(*    SSCase "x2 steps". *)
+(*     destruct H0 as [x2']. *)
+(*     exists (XApp x1 x2'). *)
+(*     apply ESApp2; auto. *)
+
+(*   SCase "x1 steps". *)
+(*    destruct H as [x1']. *)
+(*    exists (XApp x1' x2). *)
+(*    apply ESApp1; auto. *)
+(* Qed. *)
