FiatFormal/Language/SubstExistential.v
@@ -1,0 +1,139 @@
+
+Require Import FiatFormal.Language.TyJudge.
+Require Import FiatFormal.Language.SubstTypeType.
+
+(* Substitution lemma for substituting ADT contents into ADTs.
+   This is unnecessary if we further restrict ADTs such that method bodies may
+   not contain references to previously-bound ADTs.
+
+   Note that substituting a type into an expression can instantiate
+   type variables, so we also need to perform the substitution
+   to the result type.
+ *)
+
+Theorem subst_exist_exp
+  : forall ke te t1 kr tr x1 t2 x,
+    KIND ke tr kr
+    -> TYPE ke te x1 (substTT 0 tr t1)
+    -> TYPE (ke :> kr) (te :> t1) x t2
+    -> TYPE ke te (substTX 0 tr (substXX 0 x1 x)) t2.
+Proof.
+  intros. gen ke te t1 kr tr x1 t2.
+  induction x; intros; simpl.
+  Case "XVar".
+  lift_cases.
+
+(* Substitution lemma for substituting ADT contents into ADTs.
+   This is unnecessary if we further restrict ADTs such that method bodies may
+   not contain references to previously-bound ADTs.
+
+   Note that substituting a type into an expression can instantiate
+   type variables, so we also need to perform the substitution
+   to the result type.
+ *)
+
+(* Not clear that this particular statement is what I want *)
+Theorem subst_exist_adt
+  : forall ke te t1 kr tr x1 t2 ad,
+    KIND ke tr kr (* well-kinded rep type *)
+    -> TYPE ke te x1 (substTT 0 tr t1) (* existential well-typed *)
+    -> TYPEADT (ke :> kr) (te :> t1) ad t2
+    -> TYPEADT ke te (substTADT 0 tr (substXADT 0 x1 ad)) t2.
+Proof.
+Abort.
+
+(* Main substitution lemma for substituting ADT contents into program.
+   If an ADT's methods implement their abstract interfaces,
+   substituting method bodies and representation types in program
+   preserves type.
+
+   Note that substituting a type into an expression can instantiate
+   type variables, so we also need to perform the substitution
+   to the result type.
+ *)
+
+Theorem subst_exist_prog
+  : forall ke te t1 kr tr x1 t2 p,
+    KIND ke tr kr (* well-kinded rep type *)
+    -> TYPE ke te x1 (substTT 0 tr t1) (* existential well-typed *)
+    -> TYPEPROG (ke :> kr) (te :> t1) p t2 (* program well-typed with extended contexts *)
+    -> TYPEPROG ke te (substTP 0 tr (substXP 0 x1 p)) t2.
+Proof.
+Abort.
+
+Theorem subst_exist_prog_ix
+  : forall ix ix' ke te k t tr t2 x1 p,
+    get ix ke = Some k
+    -> get ix' te = Some t
+    -> KIND (delete ix ke) tr k
+    -> TYPEPROG ke te p t2
+    (* NOTE: the liftTT-ing for taur below shouldn't be necessary, just not sure where the simple condition on rep types should ultimately be stated *)
+    -> TYPE (delete ix ke) (delete ix' te) x1 (substTT 0 tr t)
+    -> TYPEPROG (delete ix ke) (delete ix' te) (substTP 0 tr (substXP 0 x1 p)) t2.
+Proof.
+Abort.
+  (* intros. *)
+  (* gen ix ix' ke te k. (* TODO: ask why gen fails with all idents in a single invocation *) *)
+  (* gen t tr t2 x1. *)
+  (* induction p; intros. *)
+  (* Case "PLet". *)
+  (* simpl; destruct a; simpl. *)
+  (* eapply TYLet. *)
+  (* SCase "ADT". *)
+
+(* Theorem subst_type_exp_ix *)
+(*   : forall ix ke te x1 t1 t2 k2, *)
+(*     get ix ke = Some k2 *)
+(*     -> TYPE ke  te x1 t1 *)
+(*     -> KIND (delete ix ke)  t2 k2 *)
+(*     -> TYPE (delete ix ke)     (substTE ix t2 te) *)
+(*            (substTX ix t2 x1) (substTT ix t2 t1). *)
+(* Proof. *)
+
+(*  intros. gen ix ke te t1 t2 k2. *)
+(*  induction x1; intros; simpl; inverts H0; eauto. *)
+
+(*  Case "XVar". *)
+(*   apply TYVar. *)
+(*   unfold substTE. eapply get_map. auto. *)
+(*   eapply subst_type_type_ix; eauto. *)
+
+(*  Case "XLAM". *)
+(*   simpl. apply TYLAM. *)
+(*   rewrite delete_rewind. *)
+(*   rewrite (liftTE_substTE 0 ix). *)
+(*   eapply IHx1; eauto. *)
+(*    apply liftTT_weaken. auto. *)
+
+(*  Case "XAPP". *)
+(*   rewrite (substTT_substTT 0 ix). *)
+(*   apply TYAPP. *)
+(*    simpl. eapply (IHx1 ix) in H6; eauto. *)
+(*    simpl. eapply subst_type_type_ix; eauto. *)
+
+(*  Case "XLam". *)
+(*   simpl. apply TYLam. *)
+(*   eapply subst_type_type_ix; eauto. *)
+(*   unfold substTE. rewrite map_rewind. *)
+(*   assert ( map (substTT ix t2) (te :> t) *)
+(*          = substTE ix t2 (te :> t)). auto. *)
+(*   rewrite H0. *)
+(*    eapply IHx1; eauto. *)
+
+(*  Case "XApp". *)
+(*   eapply TYApp. *)
+(*    eapply IHx1_1 in H6; eauto. *)
+(*    eapply IHx1_2 in H8; eauto. *)
+(* Qed. *)
+
+(* Theorem subst_type_value *)
+(*  :  forall ke te x1 t1 t2 k2 *)
+(*  ,  TYPE (ke :> k2) te x1 t1 *)
+(*  -> KIND ke  t2 k2 *)
+(*  -> TYPE ke                (substTE 0 t2 te) *)
+(*          (substTX 0 t2 x1) (substTT 0 t2 t1). *)
+(* Proof. *)
+(*  intros. *)
+(*  assert (ke = delete 0 (ke :> k2)). auto. rewrite H1. *)
+(*  eapply subst_type_exp_ix; simpl; eauto. *)
+(* Qed. *)
